nameless-w/Scoping.v
@@ -1,0 +1,157 @@
+Require Import Prelude.
+Require Import Expr.
+
+(* This is the right way to define functions :) *)
+Notation "( && b )" := (fun b' => b' && b).
+Fixpoint closed_at (l : nat) (e : exp) : bool.
+  destruct e; 
+  repeat match goal with
+           | [i : var |- _] => exact: (i < l)
+           | [e : {bind exp} |- _] => apply (closed_at l.+1) in e; apply (&& e)
+           | [e : exp |- _] => apply (closed_at l) in e; apply (&& e)
+           | _ => exact: true
+         end.
+Defined.
+
+(* While we're at it *)
+Ltac mk_size T f :=
+  repeat match goal with [e : T |- _] => apply f in e; apply (+ e) | _ => exact: 1 end.
+      
+Fixpoint term_size (e : exp) : nat.
+  destruct e; mk_size exp term_size.
+Defined.
+
+Notation closed := (closed_at 0).
+
+Notation closed_sub l sigma := (forall i, i < l -> sigma i = Bind i).
+Lemma closed_up : forall l sigma, closed_sub l sigma -> closed_sub l.+1 (up sigma).
+  intros. destruct i; asimpl; eauto. rewrite H; eauto. Qed.
+
+Tactic Notation "destr" "bands" := 
+  repeat match goal with
+           | [H: _ && _|-_] => apply andb_prop in H; destruct H
+           | [H: _ && _ = true |- _] => apply andb_prop in H; destruct H
+         end.
+
+(* This proof is gross for stupid reasons - fix later *)
+Hint Resolve andb_true_intro.
+Lemma closed_lift : forall e i j, i <= j -> closed_at i e -> closed_at j e.
+  induction e; intros; simpl in *; try reflexivity; unfold is_true in *;
+  apply leq_trans with (n := i) ||
+    (destr bands;
+    repeat match goal with [H : forall i j : nat, _ |- _] => extend (H i j); extend (H i.+1 j.+1) end);
+    auto 10.
+Qed.
+
+(* Hint Resolve le_pred le_S_n le_0_n le_n_S. *)
+(* Hint Rewrite leq_subLR leq_subr leq_sub2r ltnS. *)
+
+Lemma closed_under : forall i j sigma, i <= j -> closed_sub j sigma -> closed_sub i sigma.
+Proof. induction i; intros; try solve by inversion. apply H0. eapply leq_trans; eauto. Qed.
+
+Hint Resolve closed_up.
+Lemma closed_at_sub_id : forall e i sigma, closed_sub i sigma -> closed_at i e -> e.[sigma] = e.
+  induction e; intros i sigma Hsig; extend (closed_up _ _ Hsig); 
+  intros; simpl in *; unfold is_true in *;
+  repeat match goal with [H : _ && _ = true |- _] => apply andb_prop in H; destr_ands end;
+  f_equal; eauto.
+Qed.
+
+Hint Rewrite closed_at_sub_id using assumption.
+
+Lemma sub_0 : forall sigma, closed_sub 0 sigma. intros; solve by inversion. Qed.
+
+Notation sub_vars i j sigma := (forall v, v < i -> closed_at j (sigma v)).
+
+Hint Rewrite ltn_add2l.
+Notation upnren := (fun n => iterate upren n).
+
+Hint Resolve iterate_S iterate_0.
+
+Notation mono sigma := (forall i j, i < j -> sigma i < sigma j).
+Lemma upren_mono_less : forall v sigma, mono sigma -> upren sigma v <= sigma v. induction v; simpl; intros; auto. Qed.
+Lemma wk_mono : forall k, mono (+k). intros; autorewrite with core; auto. Qed.
+Lemma upren_mono : forall sigma, mono sigma -> mono (upren sigma). destruct i,j; try solve by inversion; simpl; autorewrite with core in *; auto. Qed.
+
+Lemma iterate_preserves A P (f : A -> A) : (forall a, P a -> P (f a)) -> forall n a, P a -> P (iterate f n a).
+Proof. induction n; intros; rewrite ?iterate_S ?iterate_0; auto. Qed.
+  
+Hint Resolve upren_mono_less wk_mono upren_mono.
+Hint Rewrite upren_mono_less wk_mono upren_mono.
+
+Lemma upnren_mono : forall n sigma, mono sigma -> mono (upnren n sigma). intros n sigma. apply iterate_preserves; auto. Qed.
+Hint Resolve upnren_mono.
+Lemma upnren_mono_less : forall n v sigma, mono sigma -> upnren n sigma v <= sigma v.
+Proof. induction n; intros; rewrite ?iterate_S; auto. apply leq_trans with (n := upnren n sigma v); auto. Qed.
+Hint Resolve upnren_mono_less.
+
+Hint Rewrite Bool.orb_false_r Bool.orb_true_iff.
+Hint Rewrite Bool.andb_negb_r Bool.andb_true_iff.
+Hint Resolve andb_prop Bool.orb_prop.
+
+Hint Rewrite up_upren_n_internal up_upren_internal using auto.
+Hint Resolve up_upren_n_internal up_upren_internal.
+Hint Resolve andb_true_intro.
+
+Notation sub_eq sigma tau := (forall v, sigma v = tau v).
+Lemma up_resp_eq : forall sigma tau, sub_eq sigma tau -> sub_eq (up sigma) (up tau). destruct v; asimpl; f_equal; auto. Qed.
+Hint Resolve up_resp_eq.
+Lemma sub_vars_tms : forall e sigma tau, sub_eq sigma tau -> e.[sigma] = e.[tau]. induction e; intros; simpl; f_equal; auto. Qed.
+Canonical sub_eq_refl : reflexive (var -> exp) (fun sigma tau => sub_eq sigma tau). constructor. Qed.
+
+Hint Rewrite sub_vars_tms using auto.
+Hint Resolve sub_vars_tms.
+Lemma wk_upn : forall e d i j, closed_at d e -> closed_at (i + d) e.[upn j (wk i)].
+  move=>e d i j. 
+  replace e.[upn j (wk i)] with e.[ren (upnren j (+ i))] by (apply sub_vars_tms; autorewrite with core; auto).
+  move:d i j.
+  induction e; intros; auto;
+  try (unfold is_true in *; simpl in *; autorewrite with core in *; destr_logic; 
+       try (rewrite <- iterate_S; replace (i + d).+1 with (i + d.+1));
+       auto; fail).
+  { simpl in *. induction j; simpl. 
+    { unfold iterate; simpl. autorewrite with core in *; auto. }
+    { rewrite iterate_S. destruct v; simpl in *.
+      { destruct j; unfold iterate in *; simpl in *; induction i; auto. }
+      { assert ((upnren j (+i) v) <= i + v) by auto.
+        assert (i + v.+1 < i + d) by (autorewrite with core; auto).
+        replace (i + v.+1) with ((i + v).+1) in H1 by auto.
+        apply leq_ltn_trans with (n := (i + v).+1); auto. }}
+  }
+Qed.
+
+Hint Resolve wk_upn.
+
+Lemma sub_wk_vars : forall i j, sub_vars i (j + i) (wk j). intros; simpl; autorewrite with core; auto. Qed.
+Lemma sub_up_vars : forall i j sigma, sub_vars i j sigma -> sub_vars i.+1 j.+1 (up sigma). 
+Proof. intros. destruct v; asimpl; auto.
+  change (wk 1) with (upn 0 (wk 1)).
+  change j.+1 with (1 + j). apply wk_upn. auto.
+Qed.
+
+Hint Resolve sub_wk_vars sub_up_vars.
+Tactic Notation "htry" :=
+  repeat match goal with
+             [H: ?P -> _, H2 : ?P |- _] => extend (H H2)
+           | [H1: forall e, _, H2 : _ |- _] => 
+             extend (H1 _ H2) || extend (H1 _ _ H2)
+         end.
+
+Lemma sub_vars_corr : forall e i j sigma, sub_vars i j sigma -> closed_at i e -> closed_at j e.[sigma].
+Proof. move=>e i j sigma Hs He.
+  move: i He j sigma Hs.
+  induction e; intros; simpl; rewrite asms; auto;
+  simpl in *; unfold is_true in *; destr bands; try apply sub_up_vars; eassumption || auto.
+Qed.
+
+Hint Resolve sub_vars_corr.
+
+Lemma closed_wk : forall e n, closed_at n e -> closed_at n.+1 e.[wk 1]. intros. change n.+1 with (1 + n). eapply sub_vars_corr; eauto. Qed.
+
+Lemma closed_sub_id : forall e sigma, closed e -> e.[sigma] = e.
+Proof. intros; apply closed_at_sub_id with (i := 0); intros; solve by inversion || auto. Qed.
+
+(* Axiom consts_wf : forall nm t, const_tys nm = Some t -> closed t. *)
+(* Axiom conv_sub : forall sigma t t', conv t t' -> conv t.[sigma] t'.[sigma]. *)
+
+(* Theorem sub_welldef sigma Delta Gamma : [Delta |+ sigma +| Gamma] -> forall t T, [Gamma |+ t :< T] -> [Delta |+ t.[sigma] :< T.[sigma]]. *)
