nameless-w/Typing.v
@@ -29,14 +29,15 @@ Definition imax (i j : nat) := match j with 0 => 0 | _ => max i j end.
 (*     | (Sum A B), Sort k => exists i j, [Gamma |+ A :< Sort i] /\ [Gamma |+ B :< Sort j] /\ i < k /\ j < k *)
 (*   end *)
 (* where "[ C |+ e :< t ]" := (has_type C e T). *)
+
 Inductive has_type (Gamma : list exp) : exp ->  exp -> Prop :=
   T_bind : forall i, i < length Gamma -> [Gamma |+ Bind i :< dget Gamma i]
 | T_free : forall nm t, const_tys nm = Some t -> [Gamma |+ Free nm :< t]
 | T_sort : forall s, [Gamma |+ Sort s :< Sort s.+1]
-(* | T_cumu : forall i j, [Gamma |+ i :< Sort j] -> [Gamma |+ i :< Sort j.+1] *)
+| T_cumu : forall i j, [Gamma |+ i :< Sort j] -> [Gamma |+ i :< Sort j.+1]
 (* | T_set : [Gamma |+ Sort set :< Sort typ] *)
 | T_pi : forall A B u1 u2, [Gamma |+ A :< Sort u1] -> [(A :: Gamma) |+ B :< Sort u2] -> [Gamma |+ (A :>> B) :< Sort (imax u1 u2)]
-| T_lam : forall A B b, [(A :: Gamma) |+ b :< B] -> [Gamma |+ (A :#> b) :< (A :>> B)]
+| T_lam : forall A B b, [(A :: Gamma) |+ b :< B] -> [Gamma |+ (Lam b) :< (A :>> B)]
 | T_app : forall A B f a, [Gamma |+ f :< (A :>> B)] -> [Gamma |+ a :< A] -> [Gamma |+ (f :$: a) :< B.[a/]]
 | T_sig :  forall A B u1 u2, [Gamma |+ A :< Sort u1] -> [(A :: Gamma) |+ B :< Sort u2] -> [Gamma |+ Sigma A B :< Sort (imax u1 u2)]
 | T_smk : forall A B a b, [Gamma |+ a :< A] -> [Gamma |+ b :< B.[a/]] -> [Gamma |+ S_mk a b :< Sigma A B]
@@ -47,27 +48,38 @@ Inductive has_type (Gamma : list exp) : exp ->  exp -> Prop :=
 | T_inl : forall A B a, [Gamma |+ a :< A] -> [Gamma |+ Sum_inl a :< Sum A B]
 | T_inr : forall A B b, [Gamma |+ b :< B] -> [Gamma |+ Sum_inr b :< Sum A B]
 | T_split : forall P A B a b ab,
-            forall n, [(Sum A B :: Gamma) |+ P :< Sort n] ->
+            (* forall n, [(Sum A B :: Gamma) |+ P :< Sort n] -> *)
               (* [(Sum A B :: Gamma) |+ P] -> *) 
                  [(    A   :: Gamma) |+ a              :< P.[Sum_inl (Bind 0) .: wk 1]] ->
                  [(      B :: Gamma) |+ b              :< P.[Sum_inr (Bind 0) .: wk 1]] ->
-                 [            Gamma  |+ Split P a b ab :< P.[ab/]]
+                 (* [            Gamma  |+ Split P a b ab :< P.[ab/]] *)
+                 [            Gamma  |+ Split a b ab   :< P.[ab/]]
                      
 (* | T_Unit : [Gamma |+ Unit :< Sort set] *)
 | T_unit : [Gamma |+ unit :< Unit]
 
 (* | T_Mu  : forall D, [Gamma |+ Mu D :< Sort set] *)
-| T_Wrap : forall d D, [Gamma |+ d :< D_efunc D (Mu D)] -> [Gamma |+ Wrap d :< Mu D]
-| T_Unwrap : forall d D, [Gamma |+ d :< Mu D] -> [Gamma |+ Unwrap d :< D_efunc D (Mu D)]
+(* | T_Wrap : forall d D, [Gamma |+ d :< D_efunc D (Mu D)] -> [Gamma |+ Wrap d :< Mu D] *)
+(* | T_Unwrap : forall d D, [Gamma |+ d :< Mu D] -> [Gamma |+ Unwrap d :< D_efunc D (Mu D)] *)
 | T_mu : forall D C a d, 
          forall n, [(Mu D :: Gamma) |+ C :< Sort n] ->
            (* [(Mu D :: Gamma) |+ C] -> *)
-              [Gamma   |+ a :< (D_efunc D (Mu D) :>> All n D C.[up (wk 1)] (Bind 0) :>> C.[Wrap (Bind 1) .: wk 2])] ->
+              [Gamma   |+ a :< (D_efunc D (Mu D) :>> All D C.[up (wk 1)] (Bind 0) :>> C.[Bind 1 .: wk 2])] ->
               [Gamma   |+ d :< Mu D] ->
-              [Gamma   |+ mu D C a d :< C.[d/]]
+              [Gamma   |+ mu D a d :< C.[d/]]
 
 | T_conv : forall A A', conv A A' -> forall a, [Gamma |+ a :< A] -> [Gamma |+ a :< A']
 where "[ C |+ e :< t ]" := (has_type C e t).
+
+Fixpoint has_type_rec (Gamma : list exp) (e : exp) (T : exp) : Prop :=
+  match e with
+    | Bind i => (i < ⟦Gamma⟧) /\ conv T (dget Gamma i)
+    | Free nm => exists t, const_tys nm = Some t /\ conv T t
+    | Sort i => exists j, i < j /\ conv T (Sort j)
+    | A :>> B => exists i j k, has_type_rec Gamma A (Sort i) /\ has_type_rec (A :: Gamma) B (Sort j) /\ k > imax i j /\ conv T (Sort k)
+    | Lam b => exists A B, has_type_rec (A :: Gamma) b B /\ conv T (A :>> B)
+    | _ => False
+  end.
 (* with is_type (Gamma : list exp) : exp -> Prop := *)
 (*   T_typ : forall e, [Gamma |+ e :< Typ] -> [Gamma |+ e] *)
 (* | T_pi : forall A B, [Gamma |+ A] -> [(A :: Gamma) |+ B] -> [Gamma |+ Pi A B] *)
